using invariants in Hazel

theories/case_studies/invariant_test_hazel.v
@@ -11,6 +11,7 @@ Definition invN : namespace := nroot .@ "inv".
 
 Definition inner (l: loc): iProp Σ := ∃ n, l ↦ n.
 
+
 Definition MyInv (l: loc) := inv invN (inner l).
 
 Global Instance MyInv_Persistent (l: loc): Persistent (MyInv l).
@@ -20,6 +21,82 @@ Qed.
 
 Definition setone : val := (λ: "l",
   "l" <- #1)%V.
+  
+Definition program : val := (λ: <>,
+  let: "l" := ref #0 in
+  setone "l")%V.
+  
+Definition sub_redexes_are_values (e : expr) :=
+  ∀ K e', e = fill K e' → to_val e' = None → K = [].
+
+Definition head_atomic (a : atomicity) (e : expr) : Prop :=
+  ∀ σ e' σ' ,
+    head_step e σ e' σ' →
+    if a is WeaklyAtomic then irreducible e' σ' else is_Some (to_val e').
+
+Lemma ectx_language_atomic a e :
+  head_atomic a e → sub_redexes_are_values e → Atomic a e.
+Proof.
+  intros Hatomic_step Hatomic_fill σ e' κ σ' efs H.
+  unfold language.prim_step in H. simpl in H. unfold prim_step' in H.
+  destruct κ, efs; try by destruct H.
+  destruct H as [K e1' e2' -> -> Hstep].
+  assert (K = []) as -> by eauto 10 using val_head_stuck.
+  simpl fill. simpl fill in Hatomic_step.
+  eapply Hatomic_step. by apply Hstep.
+Qed.
+
+Lemma fill_val2 (k : ectx) (e: expr) :
+  is_Some (to_val (fill k e)) → is_Some (to_val e).
+Proof.
+  intros (v & [-> ->]%fill_val).
+  simpl. done.
+Qed.
+
+Lemma ectxi_language_sub_redexes_are_values e :
+  (∀ Ki e', e = fill Ki e' → is_Some (to_val e')) →
+  sub_redexes_are_values e.
+Proof.
+  intros Hsub K e' ->. destruct K as [|Ki K _] using @rev_ind=> //=.
+  intros []%eq_None_not_Some. eapply fill_val2, Hsub. by rewrite /= fill_app.
+Qed.
+
+Local Ltac solve_atomic :=
+  apply ectx_language_atomic;
+  [inversion 1; naive_solver
+    |apply ectxi_language_sub_redexes_are_values; intros [] **; naive_solver].
+
+Lemma fill_no_value (k: ectx) (e: expr) (v: val) :
+  to_val e = None → fill k e = v → False.
+Proof.
+  intros Hv Hfill.
+  specialize (fill_not_val k _ Hv) as Hfill'.
+  rewrite Hfill in Hfill'.
+  simpl in Hfill'. discriminate Hfill'.
+Qed.
+
+Global Instance store_atomic v1 v2 : Atomic StronglyAtomic (Store (Val v1) (Val v2)).
+Proof. 
+  apply ectx_language_atomic.
+  - inversion 1. naive_solver. 
+  - unfold sub_redexes_are_values.
+    intros [] **. naive_solver.
+    exfalso.
+    simpl in H. destruct f; simpl in H; try discriminate H.
+    inversion H. apply (fill_no_value l e' v1 H0). symmetry. apply H2.
+    inversion H. apply (fill_no_value l e' v2 H0). symmetry. apply H3.
+Qed.
+
+Global Instance load_atomic v : Atomic StronglyAtomic (Load (Val v)).
+Proof.
+  apply ectx_language_atomic.
+  - inversion 1. naive_solver.
+  - unfold sub_redexes_are_values.
+    intros [] **. naive_solver.
+    exfalso.
+    simpl in H. destruct f; simpl in H; try discriminate H.
+    inversion H. apply (fill_no_value l e' v H0). symmetry. apply H2.
+Qed.
 
 Lemma ewp_setone (l: loc): 
   MyInv l ⊢ EWP (setone #l) {{_, True}}.
@@ -27,45 +104,55 @@ Proof.
   iIntros "HInv". rewrite /setone. ewp_pure_steps.
   rewrite /MyInv /inner.
   assert (H: Atomic StronglyAtomic (Store (LitV l) (LitV (Zpos xH)))).
-    by admit.
+    by apply _.
+  Locate StronglyAtomic.
   iApply (@ewp_atomic _ _ ⊤ (⊤ ∖ ↑invN) (Store (LitV l) (LitV (Zpos xH))) _ _ _ H). 
-  iMod (inv_acc with "HInv") as "(HInv1 & HInv2)".
+  iMod (inv_acc with "HInv") as "((%n & Hl) & Hclose)".
   done.
-  iDestruct "HInv1" as "[%n Hl]".
+  iModIntro.
   iApply (ewp_store with "Hl").
-  iIntros "!> !> Hl !>".
+  iIntros "!> Hl !>".
   iApply (fupd_elim (⊤ ∖ ↑invN) ⊤ ⊤ True True).
-  iIntros "e !>". done.
-  iApply "HInv2". iNext. iExists #1. done.
+    by iIntros "_ !>". 
+  iApply "Hclose". iNext. iExists #1. done.
+Restart.
+  iIntros "HInv". rewrite /setone. ewp_pure_steps.
+  rewrite /MyInv /inner.
+  assert (H: Atomic StronglyAtomic (Store (LitV l) (LitV (Zpos xH)))).
+    by apply _.
+  Locate StronglyAtomic.
+  iApply (@ewp_atomic _ _ ⊤ (⊤ ∖ ↑invN) (Store (LitV l) (LitV (Zpos xH))) _ _ _ H). 
+  iMod (inv_acc with "HInv") as "((%n & Hl) & Hclose)".
+  done.
+  iModIntro.
+  iApply (ewp_store with "Hl").
+  iIntros "!> Hl !>".
+  iApply "Hclose".
 Qed.
   
-  (* Unset Printing Notations. *)
-(*
-"Hl" : ▷ l ↦ n
---------------------------------------∗
-|={⊤ ∖ ↑invN}=> ▷ (∃ n0 : val, l ↦ n0) ∗ (|={⊤}=> EWP #l <- #1 {{ _, True }}) 
-*)
-
-(fupd (difference top (up_close invN)) (difference top (up_close invN))
-     (bi_sep (bi_later (bi_exist (fun n0 : val => mapsto l (DfracOwn (pos_to_Qp xH)) n0)))
-        (fupd top top
-           (ewp_def top (Store (LitV l) (LitV (Zpos xH))) iEff_bottom iEff_bottom
-              (fun _ : val => bi_pure True)))))
-
-  iInv "HInv" as (n) "Hl" "Hclose".
-(* 
-"Hl" : ▷ l ↦ n
-"Hclose" : ▷ (∃ n0 : val, l ↦ n0) ={⊤ ∖ ↑invN,⊤}=∗ emp
---------------------------------------∗
-|={⊤ ∖ ↑invN,⊤}=> EWP #l <- #1 {{ _, True }} 
-*)
-
-
-Lemma allocate_MyInv: 
-  ⊢ |==> ∃ l, MyInv l.
+Lemma allocate_MyInv (l: loc) (n: nat): 
+  (l ↦ #n) ⊢ |={⊤}=> MyInv l.
 Proof.
-  (* iInv () *)
-(* Goal ∀ l, MyInv  *)
-Admitted.
+  Check inv_alloc.
+  iIntros "Hl".
+  rewrite /MyInv.
+  iMod (inv_alloc invN ⊤ (inner l) with "[-]") as "#HInv".
+  { iNext. rewrite /inner. by iExists #n. }
+  done.
+Qed.
+
+Lemma ewp_program: 
+  ⊢ EWP (program #()) {{_, True}}.
+Proof.
+  iIntros. rewrite /program.
+  ewp_pure_steps.
+  ewp_bind_rule. simpl.
+  iApply ewp_alloc. iIntros "!> %l Hl".
+  iMod (allocate_MyInv l 0 with "Hl") as "#HInv".
+  iModIntro. ewp_pure_steps.
+  by iApply ewp_setone.
+Qed.
 
 End name.
+
+Print Assumptions ewp_program.
